WIP

theories/common.v
@@ -5,6 +5,7 @@ From Deque Require Import tick.
 (* Section notations *)
 Notation "⋅ x" := [x] (at level 60).
 Definition nonempty {A : Type} (x : list A) := ~(x = []).
+Notation "[4..6]" := [4; 5; 6].
 Notation "[3..6]" := [3; 4; 5; 6].
 Notation "[2..6]" := [2; 3; 4; 5; 6].
 Notation "[1..7]" := [1; 2; 3; 4; 5; 6; 7].
@@ -123,6 +124,10 @@ Section configurations.
     | suffix_only : forall s, s ∈ [1..8] -> five_tuple_configuration 0 0 0 0 s
     | has_middle : forall p ld rd s, p ∈ [3..6] -> s ∈ [3..6] -> five_tuple_configuration p ld 2 rd s.
 
+  (* Five-tuple configuration for calling naive_pop *)
+  Inductive pop_configuration : nat -> nat -> nat -> nat -> nat -> Prop :=
+    | pop_suffix_only : forall s, s ∈ [1..8] -> pop_configuration 0 0 0 0 s
+    | pop_has_middle : forall p ld rd s, p ∈ [4..6] -> s ∈ [3..6] -> pop_configuration p ld 2 rd s.
 
   Inductive colour : Set :=
     | green | red | very_red.
@@ -160,6 +165,13 @@ Section algorithms.
       let: y := Snd "TMP2" in
       v)%E
      (at level 190, x,y at next level, u at next level, v at next level, only parsing).
+
+  Notation "'let:3' ( v , w , x ) := U 'in' V"
+    := (let: "TMP3" := U in
+        let:2 ("TMP3", x) := "TMP3" in
+        let:2 (v, w) := "TMP3" in
+        V)%E
+      (at level 190, v,w,x at next level, U at next level, V at next level, only parsing).
 
   Notation "'let:5' ( v , w , x , y , z ) := U 'in' V"
     := (let: "TMP5" := U in
@@ -234,5 +246,157 @@ Section algorithms.
       else push ("p2'", empty, empty_buffer) "rd2'" in
     SOME (ref ("pr1", "ld1''", "middle", "rd2''", "sf2"))
     end end.
+
+  Definition naive_pop : val :=
+    λ: "d",
+    let:5 ("pr", "ld", "md", "rd", "sf") := "d" in
+    if: bsize "md" = #0%nat then (
+      let:2 ("x", "sf'") := bpop "sf" in
+      ("x", SOME (ref ("pr", "ld", "md", "rd", "sf'")))
+    ) else (
+      let:2 ("x", "pr'") := bpop "pr" in
+      ("x", SOME (ref ("pr'", "ld", "md", "rd", "sf")))
+    ).
+
+  Definition inspect_first : val :=
+    λ: "d", Fst (naive_pop "d").
+
+  (* TODO: lookup actual not *)
+  Let not : val := λ: "b", if: "b" then (#0 = #1) else (#0 = #0).
+
+  Definition first_nonempty : val :=
+    λ: "tr",
+      let:3 ("first", "middle", "last") := "tr" in
+      if: not (bsize "first" = #0%nat)%E
+        then SOME "first"
+      else if: not (bsize "last" = #0%nat)
+        then SOME "last"
+      else NONE.
+
+  Definition pop : val :=
+    rec: "pop" "d" :=
+    tick #();;
+    match: "d" with NONE => "unreachable"
+    | SOME "ptr" =>
+    let: "d" := !"ptr" in
+    let:5 ("prefix", "left", "middle", "right", "suffix") := "d" in
+    let: "d'" :=
+    if: (bsize "middle" = #0%nat) || not (bsize "prefix" = #3%nat) then "d" else (
+      (* assert: bsize "prefix" = #3%nat *)
+      match: "left" with
+        SOME "left" =>
+        let: "left" := !"left" in
+        let: "t" := inspect_first "left" in
+        let:2 ("t", "l") :=
+          let:3 ("first", "child", "last") := "t" in
+          let: "fn_result" := first_nonempty "t" in
+          match: "fn_result" with
+            SOME "b" =>
+            if: bsize "b" = #3%nat || ("child" = NONE) then
+              naive_pop "left"
+            else
+              "pop" (SOME (ref "left"))
+          | NONE => "UNREACHABLE"
+          end in
+        let:3 ("x", "d'", "y") := "t" in
+        let: "x_len" := bsize "x" in
+        let: "y_len" := bsize "y" in
+        if: "x_len" = #3%nat then (
+          let:2 ("a", "x'") := bpop "x" in
+          let: "p'" := binject "prefix" "a" in
+          let: "triple" := ("x'", "d'", "y") in
+          let: "ld'" := push "triple" "l" in
+          ("p'", "ld'", "middle", "right", "suffix")
+        ) else if: "x_len" = #2%nat then (
+          let: "p'" := inject_whole_buffer inject "prefix" "x" in
+          if: ("d'" = NONE) && (bsize "y" = #0%nat) then
+            ("p'", "l", "middle", "right", "suffix")
+          else
+            let: "triple" := ("y", empty, empty_buffer) in
+            let: "l'" := dconcat "d'" (push "triple" "l") in
+            ("p'", "l'", "middle", "right", "suffix")
+        ) else if: ("x_len" = #0%nat) && ("y_len" = #3%nat) then (
+          (* x is empty therefore d' is empty *)
+          let:2 ("a", "y'") := bpop "y" in
+          let: "p'" := binject "prefix" "a" in
+          let: "triple" := ("x", "d'", "y'") in
+          let: "ld'" := push "triple" "l" in
+          ("p'", "ld'", "middle", "right", "suffix")
+        ) else if: ("x_len" = #0%nat) && ("y_len" = #2%nat) then (
+          let: "p'" := inject_whole_buffer inject "prefix" "y" in
+          ("p'", "l", "middle", "right", "suffix")
+        ) else
+          "UNREACHABLE"
+      | NONE =>
+        match: "right" with
+          SOME "right" =>
+          let: "right" := !"right" in
+          let: "t" := inspect_first "right" in
+          let:2 ("t", "r") :=
+            let: "fn_result" := first_nonempty "t" in
+            match: "fn_result" with
+              SOME "b" =>
+              if: (bsize "b" = #3%nat) || not ("child" = NONE) then
+                naive_pop "right"
+              else
+                "pop" (SOME (ref "right"))
+            | NONE => "UNREACHABLE"
+            end in
+          let:3 ("x", "d'", "y") := "t" in
+          let: "x_len" := bsize "x" in
+          let: "y_len" := bsize "y" in
+          if: "x_len" = #3%nat then (
+            let:2 ("a", "m") := bpop "middle" in
+            let: "p" := binject "prefix" "a" in
+            let:2 ("b", "x'") := bpop "x" in
+            let: "m'" := binject "m" "b" in
+            let: "triple" := ("x'", "d'", "y") in
+            let: "r'" := push "triple" "r" in
+            ("p", "left", "m'", "r'", "suffix")
+          ) else if: "x_len" = #2%nat then (
+            let: "p" := inject_whole_buffer binject "prefix" "middle" in
+            let: "r'" :=
+              if: ("d'" = NONE) && (bsize "y" = #0%nat) then
+                "r"
+              else
+                let: "triple" := ("y", empty, empty_buffer) in
+                dconcat "d'" (push "triple" "r")
+            in
+            ("p", "left", "x", "r'", "suffix")
+          ) else if: ("x_len" = #0%nat) && ("y_len" = #3%nat) then (
+            (* x is empty therefore d' is empty too *)
+            let:2 ("a", "m") := bpop "middle" in
+            let: "p" := binject "prefix" "a" in
+            let:2 ("b", "y'") := bpop "y" in
+            let: "m'" := binject "m" "b" in
+            let: "triple" := ("x", "d'", "y'") in
+            let: "r'" := push "triple" "r" in
+            ("p", "left", "m'", "r'", "suffix")
+          ) else if: ("x_len") = #0%nat && ("y_len" = #2%nat) then (
+            let: "p" := inject_whole_buffer binject "prefix" "middle" in
+            ("p", "left", "y", "right", "suffix")
+          ) else
+            "UNREACHABLE"
+        | NONE =>
+          (* is_empty left, is_empty right *)
+          if: bsize "suffix" = #3%nat then
+            let: "suffix'" := inject_whole_buffer binject "prefix" (inject_whole_buffer binject "middle" "suffix") in
+            (empty_buffer, "left", empty_buffer, "right", "suffix'")
+          else
+            let:2 ("a", "m") := bpop "middle" in
+            let: "prefix'" := binject "prefix" "a" in
+            let:2 ("a", "suffix'") := bpop "suffix" in
+            let: "middle'" := binject "m" "a" in
+            ("prefix'", "left", "middle'", "right", "suffix'")
+        end
+      end
+    )
+    in
+    (* TODO: fix OCaml code *)
+    "ptr" <- "d'";;
+    naive_pop "d'"
+    end.
+
+  Definition eject : val. Admitted.
 
 End algorithms.
